Babel/MetaLanguage/UFeatures/UWhile.v
@@ -1,0 +1,172 @@
+(** UWhile.v *)
+From Babel Require Import TerminalDogma 
+                          ExtraDogma.Extensionality
+                          EpsilonDescription
+                          SetFacility
+                          POrderFacility.
+
+From Babel Require Import Ranko
+                            ExtensionalityCharacter
+                            ClassicalCharacter.
+
+From Babel.MetaLanguage Require Import Notations
+                                        MetaType
+                                        MetaLan.
+
+From Coq Require Import Relations Classical.
+
+Set Implicit Arguments.
+Unset Strict Implicit.
+Unset Printing Implicit Defensive.
+
+(** Do not import this module. *)
+Module UWhile.
+
+
+(** Syntax *)
+
+Record syn (mT : cpo) (Hj : FlowCtrl.join mT) (syn0 : Type) := while_ {
+    flow_split : FlowCtrl.split Hj;
+    S0 : syn0;
+}.
+
+Notation M0 s := (FlowCtrl.M0 (flow_split s)).
+Notation M1 s := (FlowCtrl.M1 (flow_split s)).
+
+Notation "'While' M 'Do' s0 'End'" := (while_ M s0) : MetaLan_scope.
+
+
+(** DeSem 
+
+    Notice the application of Kleene fixpoint here.
+*)
+
+Definition while_iter (mT : cpo) (Hj : FlowCtrl.join mT) 
+    (de0 : deSem mT) (P : mT): 
+    syn Hj de0 -> mT -> mT :=
+        fun s X => ((M0 s) (⟦ S0 s ⟧ <de0> X)) ⊕[Hj] ((M1 s) P).
+
+Lemma while_iter_mono_mixin (mT : cpo) (Hj : FlowCtrl.join mT) 
+    (de0 : deSem mT) (P : mT) (s : syn Hj de0) : 
+    MonotonicFun.mixin_of (while_iter P s).
+Proof. rewrite /MonotonicFun.mixin_of /while_iter => x y Hxy.
+    transitivity (M0 s ((⟦ S0 s ⟧ < de0 >) x) ⊕[ Hj] M1 s P).
+    - apply FlowCtrl.join_monot1.
+        apply MonotonicFun.class. by reflexivity.
+    - apply FlowCtrl.join_monot0.
+        apply MonotonicFun.class.
+        by apply MonotonicFun.class.
+Qed.
+
+Canonical while_iter_mono (mT : cpo) (Hj : FlowCtrl.join mT) 
+    (de0 : deSem mT) (P : mT) (s : syn Hj de0) : [ mT ↦ᵐ mT ] :=
+    MonotonicFun (while_iter P s) (while_iter_mono_mixin P s).
+
+Lemma while_iter_conti_mixin (mT : cpo) (Hj : FlowCtrl.join mT) 
+    (de0 : deSem mT) (P : mT) (s : syn Hj de0) : 
+    ContinuousFun.mixin_of (MonotonicFun.class (while_iter P s)).
+Proof. rewrite /ContinuousFun.mixin_of => ch //=.
+    rewrite /while_iter //=.
+Admitted.
+
+Canonical while_iter_conti (mT : cpo) (Hj : FlowCtrl.join mT) 
+    (de0 : deSem mT) (P : mT) (s : syn Hj de0) : [ mT ↦ mT ] :=
+    ContinuousFun (while_iter P s) (while_iter_conti_mixin P s).
+
+
+Definition de_fun (mT : cpo) (Hj : FlowCtrl.join mT) (de0 : deSem mT) : 
+    syn Hj de0 -> mT -> mT := 
+        fun s P => KleeneFp (while_iter P s).
+
+Lemma de_fun_monot_mixin (mT : cpo) (Hj : FlowCtrl.join mT) 
+    (de0 : deSem mT) (s : syn Hj de0) : MonotonicFun.mixin_of (de_fun s).
+Proof. rewrite /MonotonicFun.mixin_of /de_fun //= => x y Hxy.
+    rewrite /KleeneFp.
+
+    (** proof by order of functions by KleeneFp. *)
+Admitted.
+
+Canonical de_fun_monot (mT : cpo) (Hj : FlowCtrl.join mT) 
+    (de0 : deSem mT) (s : syn Hj de0) : [ mT ↦ᵐ mT ] :=
+    MonotonicFun (de_fun s) (de_fun_monot_mixin s).
+
+Lemma de_fun_conti_mixin (mT : cpo) (Hj : FlowCtrl.join mT) 
+    (de0 : deSem mT) (s : syn Hj de0) : 
+        ContinuousFun.mixin_of (MonotonicFun.class (de_fun s)).
+Proof. 
+    rewrite /ContinuousFun.mixin_of //= => ch.
+    rewrite /de_fun //=.
+Admitted.
+
+Canonical de_fun_conti (mT : cpo) (Hj : FlowCtrl.join mT) 
+    (de0 : deSem mT) (s : syn Hj de0) : [ mT ↦ mT ] :=
+    ContinuousFun (de_fun s) (de_fun_conti_mixin s).
+
+Definition deSem_mixin (mT : cpo) (Hj : FlowCtrl.join mT) (de0 : deSem mT) : 
+    DeSem.mixin_of mT (syn Hj de0) :=
+{|
+	DeSem.de_fun := @de_fun mT Hj de0;
+|}.
+
+Definition deSem (mT : cpo) (Hj : FlowCtrl.join mT) (de0 : deSem mT) :=
+    DeSem (syn Hj de0) (deSem_mixin Hj de0).
+
+
+(** AxSem 
+    Note that cpoDMT is needed here.
+*)
+
+Inductive ax_sys (mT : cpoDMT) (Hj : FlowCtrl.join mT) (ax0 : axSem mT) : 
+    mT -> syn Hj ax0 -> mT -> Prop :=
+
+| RULE_LOOP (M : FlowCtrl.split Hj)
+        (s0 : ax0) (P Inv Q : mT) 
+        (H : ⊢ <ax0> { Inv } s0 { (FlowCtrl.M0 M Inv) ⊕[Hj] (FlowCtrl.M1 M Q) }) 
+        (Himp : mT ⊢ P ⇒ Inv): 
+
+            ax_sys P (While M Do s0 End) Q.
+            
+
+Definition axSem_mixin (mT : cpoDMT) (Hj : FlowCtrl.join mT) 
+    (ax0 : axSem mT) : AxSem.mixin_of mT (syn Hj ax0)
+    := @AxSem.Mixin mT _ (@ax_sys mT Hj ax0).
+
+Definition axSem (mT : cpoDMT) (Hj : FlowCtrl.join mT) (ax0 : axSem mT) 
+        : AxSem.mixin_of mT (syn Hj ax0) :=
+    AxSem (syn Hj ax0) (axSem_mixin Hj ax0).
+        
+
+
+(** VeriModS *)
+
+Definition veriModS_mixin (mT : cpoDMT) (Hj : FlowCtrl.join mT) 
+    (veriS0 : veriModS mT): 
+    VeriModS.mixin_of (axSem Hj veriS0) (deSem Hj veriS0).
+Proof. 
+    constructor. rewrite /VeriModS.axiom => [] [] Hs s0 P Q.
+    move => [] //=. intros. rewrite /de_fun.
+
+    transitivity Inv.
+    - by apply /(CpoDMT.ded_iffP (CpoDMT.mixin mT)).
+
+    apply (soundness_of veriS0) in H.
+    apply (poset_trans H).
+    rewrite /KleeneFp //=.
+
+
+    
+
+    
+
+    apply (soundness_of veriS1) in H1 => //=.
+    apply (soundness_of veriS0) in H0 => //=.
+    
+    transitivity ((⟦ s2 ⟧ < DeSem veriS0 (VeriModS.base_de veriS0) >) R).
+    - by [].
+    - by apply (DeSem.de_monot).
+Qed.
+
+Definition veriModS (mT : cpoDMT) (veriS0 veriS1 : veriModS mT) := 
+    VeriModS (syn veriS0 veriS1) (veriModS_mixin veriS0 veriS1).
+    
+End UWhile.
