Babel/POrderFacility/FixPoint.v
@@ -1,0 +1,89 @@
+(** * FixPoint.v *)
+
+From Babel Require Import TerminalDogma 
+                          ExtraDogma.Extensionality
+                          SetFacility.
+
+From Babel Require Export POrder.
+
+From Babel Require Import Ranko.POrderCharacter.
+
+From Coq Require Import Relations Arith.
+
+Set Implicit Arguments.
+Unset Strict Implicit.
+Unset Printing Implicit Defensive.
+
+
+
+(* the definition of a fixpoint *)
+Definition fp (T : poset) (f : T -> T) (x : T) : Prop := f x = x.
+
+(* set of fixpoints *)
+Definition fp_s (T : poset) (f : T -> T) : 𝒫(T) := { x | fp f x }.
+
+(* pre-fixpoint *)
+Definition pre_fp (T : poset) (f : T -> T) (x : T) : Prop := x ⊑ f x.
+
+(* pre-fixpoint set *)
+Definition pre_fp_s (T : poset) (f : T -> T) : 𝒫(T) := { x | pre_fp f x }.
+
+(* post-fixpoint *)
+Definition post_fp (T : poset) (f : T -> T) (x : T) : Prop := f x ⊑ x.
+
+(* post-fixpoint set *)
+Definition post_fp_s (T : poset) (f : T -> T) : 𝒫(T) := { x | post_fp f x }.
+
+(* fp_in_pre_fp : fp_s f ⊆ pre_fp_s f *)
+Lemma fp_in_pre_fp (T : poset) : forall f : T -> T, fp_s f ⊆ pre_fp_s f.
+Proof.
+    rewrite /subset /fp_s /fp /pre_fp_s /pre_fp => //= f x ->.
+    by reflexivity.
+Qed.
+
+(* fp_in_post_fp : fp_s f ⊆ post_fp_s f *)
+Lemma fp_in_post_fp (T : poset) : forall f : T -> T, fp_s f ⊆ post_fp_s f.
+Proof.
+    have Hdual := @fp_in_pre_fp (T †po).
+    by apply Hdual.
+Qed.
+
+
+(* a is the least fixpoint of f greater than x *)
+Definition lfp_x (T : poset) (f : T -> T) (x a : T) := 
+    least ({ y | y ∈ fp_s f /\ x ⊑ y }) a.
+
+(* a is the least fixpoint of f *)
+Definition lfp (T : poset) (f : T -> T) (a : T) := 
+    least (fp_s f) a.
+    
+(* a is the greatest fixpoint of f smaller than x *)
+Definition gfp_x (T : poset) (f : T -> T) (x a : T) := 
+    largest ({ y | y ∈ fp_s f /\ y ⊑ x }) a.
+
+
+(* a is the greatest fixpoint of f *)
+Definition gfp (T : poset) (f : T -> T) (a : T) := 
+    largest (fp_s f) a.
+
+
+
+Lemma monofun_power_chain_mixin (T : cpo) (f : [T ↦ᵐ T]) (s : 𝒫(nat)): 
+        Chain.mixin_of ((fun_power f) [<] s [>] (⊔ᶜᵖᵒ (set_em T))).
+Proof.
+    rewrite /Chain.mixin_of. porder_level.
+    clear - f.
+    case E: (x1 <= x3).
+    - left.
+Admitted.
+
+Canonical monofun_power_chain (T : cpo) (f : [T ↦ᵐ T]) (s : 𝒫(nat)) : chain T
+    := Chain ((fun_power f) [<] s [>] (⊔ᶜᵖᵒ (set_em T))) 
+            (@monofun_power_chain_mixin T f s).
+
+
+Definition KleeneFp (T : cpo) (f : [T ↦ T]) : T :=
+    ⊔ᶜᵖᵒ ((fun_power f) [<] 𝕌 [>] (⊔ᶜᵖᵒ (set_em T))).
+
+Axiom KleeneTheorem :
+    forall (T : cpo) (f : [T ↦ T]), lfp f (KleeneFp f).
